theories/CheckWf.v
@@ -60,90 +60,198 @@ Definition agda_typed_eflags : EEnvFlags :=
      cstr_as_blocks  := true;   (* The backend fully applies ctors       *)
   |}.
 
-Definition inspect {A} (a : A) : {b | a = b} := exist _ a eq_refl.
+From MetaCoq.Erasure Require Import EGlobalEnv.
+From MetaCoq.Erasure Require Import EPrimitive.
 
-Fixpoint check_fresh_global (k : kername) (decls : global_declarations) : bool :=
+From MetaCoq.Utils Require Import utils.
+From MetaCoq.Erasure.Typed Require Import ResultMonad.
+
+Import MCMonadNotation.
+
+From MetaCoq.Common Require Import Primitive.
+
+
+Section Wf.
+  Context {efl  : EEnvFlags}.
+  Variable Σ : global_context.
+
+  Definition assert (b : bool) (s : string) : (fun T => result T string) unit :=
+    if b then Ok tt else Err s.
+
+  Definition assert_some {A : Type} (b : option A) (s : string) : (fun T => result T string) unit :=
+    match b with
+    | Some _ =>  Ok tt
+    | None => Err s
+    end.
+
+  Definition result_forall {A : Type} (f : A -> (fun T => result T string) unit ) (l : list A) :=
+    List.fold_left (fun a t => a ;; f t) l (Ok tt).
+
+  Definition wf_fix_gen_ (wf : nat -> term -> (fun T => result T string) unit) k mfix idx :=
+    let k' := List.length mfix + k in
+    assert (idx <? #|mfix|) "Fixpoint index out of bounds" ;;
+    result_forall (fun d => (wf k') d.(dbody)) mfix.
+
+  Definition bool_of_result {T E : Type} (r : result T E) : bool :=
+    match r with
+    | Ok _ => true
+    | Err _ => false
+    end.
+
+  Definition has_prim_ {epfl : EPrimitiveFlags} (p : prim_val term) : (fun T => result T string) unit :=
+    match prim_val_tag p with
+    | primInt => assert has_primint "Program contains primitive integers"
+    | primFloat => assert has_primfloat "Program contains primitive floats"
+    | primArray => assert has_primarray "Program contains primitive arrays"
+    end.
+
+  (* TODO: more informative errors messages *)
+  Fixpoint wellformed (k : nat) (t : term) {struct t} : (fun T => result T string) unit :=
+    match t with
+    | tRel i => assert has_tRel "Program contains tRel" ;; assert (Nat.ltb i k) "Program not closed"
+    | tEvar ev args => assert has_tEvar "Program contains tEvar" ;; result_forall (wellformed k) args
+    | tLambda _ M => assert has_tLambda "Program contains tLambda" ;; wellformed (S k) M
+    | tApp u v =>
+      assert has_tApp "Program contains tApp" ;;
+      wellformed k u ;;
+      wellformed k v
+    | tLetIn na b b' =>
+      assert has_tLetIn "Program contains tLetIn" ;;
+      wellformed k b ;;
+      wellformed (S k) b'
+    | tCase ind c brs =>
+      assert has_tCase "Program contains tCase" ;;
+      let brs' := result_forall (fun br => wellformed (#|br.1| + k) br.2) brs in
+      wf_brs Σ ind.1 #|brs| ;;
+      wellformed k c ;;
+      brs'
+    | tProj p c =>
+      assert has_tProj "Program contains tProj" ;;
+      assert_some (lookup_projection Σ p) "Projection not found" ;;
+      wellformed k c
+    | tFix mfix idx =>
+      assert has_tFix "Program contains tFix" ;;
+      result_forall (fun t => assert ((isLambda ∘ dbody) t) "Fixpoint body is not a lambda") mfix ;;
+      wf_fix_gen_ wellformed k mfix idx
+    | tCoFix mfix idx =>
+      assert has_tCoFix "Program contains tCoFix" ;;
+      wf_fix_gen_ wellformed k mfix idx
+    | tBox => assert has_tBox "Program contains tBox"
+    | tConst kn =>
+      assert has_tConst "Program contains tConst" ;;
+      match lookup_constant Σ kn with
+      | Some d => assert (has_axioms || isSome d.(cst_body)) "Invalid axiom"
+      | _ => Err "Constant not found in environment"
+      end
+    | tConstruct ind c block_args =>
+      assert has_tConstruct "Program contains tConstruct" ;;
+      assert_some (lookup_constructor Σ ind c) "Constructor not found" ;;
+      if cstr_as_blocks then
+        match lookup_constructor_pars_args Σ ind c with
+        | Some (p, a) => assert ((p + a) == #|block_args|) "Constructor not fully applied"
+        | _ => Ok tt end
+        ;; result_forall (wellformed k) block_args
+      else assert (is_nil block_args) "Constructor args non-empty"
+    | tVar _ => assert has_tVar "Program contains tVar"
+    | tPrim p => has_prim_ p ;; assert (test_prim (fun t => bool_of_result (wellformed k t)) p) "Invalid array primitive"
+    | tLazy t => assert has_tLazy_Force "Program contains lazy/force" ;; wellformed k t
+    | tForce t => assert has_tLazy_Force "Program contains lazy/force" ;; wellformed k t
+    end.
+
+  Theorem wellformed_equiv : forall k t,
+    bool_of_result (wellformed k t) = EWellformed.wellformed Σ k t.
+  Proof.
+  Admitted.
+End Wf.
+
+
+
+
+
+Fixpoint check_fresh_global (k : kername) (decls : global_declarations) : (fun T => result T string) unit :=
   match decls with
-  | []    => true
-  | p::ds => negb (eq_kername (fst p) k) && check_fresh_global k ds
+  | []    => Ok tt
+  | p::ds => assert (negb (eq_kername (fst p) k)) "Duplicate definition" ;; check_fresh_global k ds
   end.
 
-Fixpoint check_wf_glob {efl : EEnvFlags} (decls : global_declarations) : bool :=
+Fixpoint check_wf_glob {efl : EEnvFlags} (decls : global_declarations) : (fun T => result T string) unit :=
   match decls with
-  | []    => true
-  | p::ds => check_wf_glob ds && check_fresh_global (fst p) ds && wf_global_decl ds (snd p)
+  | []    => Ok tt
+  | p::ds => check_wf_glob ds ;; check_fresh_global (fst p) ;; assert (wf_global_decl ds (snd p)) "Decl not wellformed"
   end.
 
-Definition check_wf_program {efl : EEnvFlags} (p : program) : bool :=
-  check_wf_glob (fst p) && wellformed (fst p) 0 (snd p).
+Definition check_wf_program {efl : EEnvFlags} (p : program) : (fun T => result T string) unit :=
+  check_wf_glob (fst p) ;; wellformed (fst p) 0 (snd p).
+
+(* Definition inspect {A} (a : A) : {b | a = b} := exist _ a eq_refl.
 
 (* freshness boolean check coincides with the freshness property *)
 Fixpoint check_fresh_globalP (k : kername) (decls : global_declarations)
   : reflectProp (fresh_global k decls) (check_fresh_global k decls).
 Proof.
   dependent elimination decls; simpl.
-- apply reflectP.
-  apply Forall_nil.
-- destruct (inspect (fst p == k)).
-  destruct x; rewrite e; simpl.
-  + apply reflectF => global_ds.
-    dependent elimination global_ds.
-    apply n.
-    by apply eqb_eq.
-  + destruct (check_fresh_globalP k l).
-    * apply reflectP.
-      apply Forall_cons; auto.
-      destruct (neqb (fst p) k) as [Hneq _].
-      apply Hneq.
-      by rewrite e.
-    * apply reflectF => gds.
-      by dependent elimination gds.
+  - apply reflectP.
+    apply Forall_nil.
+  - destruct (inspect (fst p == k)).
+    destruct x; rewrite e; simpl.
+    + apply reflectF => global_ds.
+      dependent elimination global_ds.
+      apply n.
+      by apply eqb_eq.
+    + destruct (check_fresh_globalP k l).
+      * apply reflectP.
+        apply Forall_cons; auto.
+        destruct (neqb (fst p) k) as [Hneq _].
+        apply Hneq.
+        by rewrite e.
+      * apply reflectF => gds.
+        by dependent elimination gds.
 Defined.
 
 (* well-formedness boolean check coincides with the wf property *)
 Fixpoint check_wf_globP {efl : EEnvFlags} (decls : global_declarations)
   : reflectProp (wf_glob decls) (check_wf_glob decls).
 Proof.
-dependent elimination decls.
-- apply reflectP.
-  apply wf_glob_nil.
-- remember (check_wf_glob l).
-  pose x := (check_wf_globP efl l).
-  rewrite <-Heqb in x.
-  destruct x; simpl; rewrite <-Heqb; simpl.
-  + remember (check_fresh_global (fst p) l).
-    pose x := (check_fresh_globalP (fst p) l).
-    rewrite <-Heqb0 in x.
-    destruct x => /=.
-    remember (wf_global_decl l (snd p)).
-    destruct b.
-    apply reflectP.
-    destruct p.
-    by constructor.
-    apply reflectF => gds.
-    dependent elimination gds.
-    simpl in Heqb1.
-    rewrite <-Heqb1 in i.
-    discriminate i.
-    apply reflectF => gds.
-    by dependent elimination gds.
-  + apply reflectF => gds.
-    by dependent elimination gds.
-Defined.
+  dependent elimination decls.
+  - apply reflectP.
+    apply wf_glob_nil.
+  - remember (check_wf_glob l).
+    pose x := (check_wf_globP efl l).
+    rewrite <-Heqb in x.
+    destruct x; simpl; rewrite <-Heqb; simpl.
+    + remember (check_fresh_global (fst p) l).
+      pose x := (check_fresh_globalP (fst p) l).
+      rewrite <-Heqb0 in x.
+      destruct x => /=.
+      remember (wf_global_decl l (snd p)).
+      destruct b.
+      apply reflectP.
+      destruct p.
+      by constructor.
+      apply reflectF => gds.
+      dependent elimination gds.
+      simpl in Heqb1.
+      rewrite <-Heqb1 in i.
+      discriminate i.
+      apply reflectF => gds.
+      by dependent elimination gds.
+    + apply reflectF => gds.
+      by dependent elimination gds.
+Defined. *)
 
 Module CheckWfExAst.
   Import ExAst.
 
-  Fixpoint check_fresh_global (k : kername) (decls : global_env) : bool :=
+  Fixpoint check_fresh_global (k : kername) (decls : global_env) : (fun T => result T string) unit  :=
     match decls with
-    | []    => true
-    | (kn,_,_)::ds => negb (eq_kername kn k) && check_fresh_global k ds
+    | []    => Ok tt
+    | (kn,_,_)::ds => assert (negb (eq_kername kn k)) "Duplicate definitions" ;; check_fresh_global k ds
     end.
 
-  Definition check_wf_typed_program {efl : EEnvFlags} (p : global_env) : bool :=
+  Definition check_wf_typed_program {efl : EEnvFlags} (p : global_env) : (fun T => result T string) unit  :=
     check_wf_glob (trans_env p).
 
-  Fixpoint check_fresh_globalP (k : kername) (decls : global_env)
+(*   Fixpoint check_fresh_globalP (k : kername) (decls : global_env)
     : reflectProp (fresh_global k decls) (check_fresh_global k decls).
   Proof.
     dependent elimination decls; simpl.
@@ -164,5 +272,5 @@ Module CheckWfExAst.
           by rewrite e.
         * apply reflectF => gds.
           by dependent elimination gds.
-  Defined.
+  Defined. *)
 End CheckWfExAst.
